pulse/ulib/experimental/Steel.PCM.Reference.fsti
@@ -55,12 +55,6 @@ val gather_atomic (#a:Type0) (#uses:_) (#p0:perm) (#p1:perm) (#v0 #v1:erased a) 
     (pts_to r p0 v0 `star` pts_to r p1 v1)
     (fun _ -> pts_to r (sum_perm p0 p1) v0)
 
-val ghost_read_refine (#a:Type0) (#uses:inames) (#p:perm) (r:ref a)
-                      (q:a -> slprop)
-  : SteelAtomic a uses unobservable
-    (h_exists (fun (v:a) -> pts_to r p v `star` q v))
-    (fun v -> pts_to r p v `star` q v)
-
 val cas (#t:eqtype)
         (#uses:inames)
         (r:ref t)
